src/lib/sparse/Kuiper.Sparse.SPMM.fsti
@@ -10,30 +10,34 @@ open Kuiper.Tensor { ctlayout }
 open Kuiper.Sparse
 open Kuiper.EMatrix
 open Kuiper.Array.Vectorized
+open Kuiper.Array2.Strided { strided_row_major, aligned_strided_row_major }
 
 inline_for_extraction noextract
 fn spmm
   (#et : Type0) {| scalar et, sized et, has_vec_cpy et |}
-  (rows shared cols : szp)
+  (rows shared cols : szp { chunk et /? cols })
   (blockItemsK : szp)
   (blockItemsX : szp)
   (blockWidth : (k : szp {
     (k * chunk et) /? blockItemsK /\
     (k * chunk sz) /? blockItemsK /\
-    k /? blockItemsX
+    (k * chunk et) /? blockItemsX
   }))
   (blockChunks : sz{SZ.v blockChunks == blockItemsX / blockWidth}) // Ver nota abajo
-  (#lB : Array2.layout shared cols)
-  (#lC : Array2.layout rows cols)
-  {| ctlayout lB, ctlayout lC |}
+  (#lB : Array2.layout shared cols) {| ctlayout lB, srmB : strided_row_major lB |}
+  (#lC : Array2.layout rows cols)   {| ctlayout lC, srmC : strided_row_major lC |}
   (gA : smatrix et (SZ.v rows) (SZ.v shared){is_global_smatrix gA})
   (#_ : squash (aligned 16 gA.elems /\ aligned 16 gA.col_ind))
   (#fA : perm)
   (row_indices : gpu_array sz rows)
   (fri : perm)
   (gB : Array2.t et lB{Array2.is_global gB})
+  (#_ : squash (aligned 16 (Array2.core gB)))
+  (#_ : squash (aligned_strided_row_major (chunk et) srmB))
   (#fB : perm)
   (gC : Array2.t et lC{Array2.is_global gC})
+  (#_ : squash (aligned 16 (Array2.core gC)))
+  (#_ : squash (aligned_strided_row_major (chunk et) srmC))
   // matriz sparse gA
   (elems : erased (lseq et gA.nnz))
   (col_ind : erased (lseq sz gA.nnz))
